Followup on renamings from project-everest/hacl-star@820d22d22

src/tls/Hashing.fst
@@ -5,7 +5,7 @@ open Mem
 
 include Hashing.Spec
 
-open FStar.HyperStack.ST 
+open FStar.HyperStack.ST
 open FStar.Bytes
 open FStar.Integers
 
@@ -14,42 +14,42 @@ module ST = FStar.HyperStack.ST
 module B = LowStar.Buffer
 
 // defining those on FStar.Bytes, not on EverCrypt's seq Uin8.t
-type hashable (a:alg) = b:bytes {length b <= maxLength a}
-type tag (a:alg) = lbytes32 (tagLen a)
+type hashable (a:alg) = b:bytes {length b <= max_input_length a}
+type tag (a:alg) = lbytes32 (Hacl.Hash.Definitions.hash_len a)
 
-// 18-08-31 pure hash specification; 
+// 18-08-31 pure hash specification;
 // renamed from [hash] already included from EverCrypt.Hash
-let h (a:alg) (b:hashable a): GTot (tag a) = 
-  let v = spec a (Bytes.reveal b) in
+let h (a:alg) (b:hashable a): GTot (tag a) =
+  let v = Spec.Hash.hash a (Bytes.reveal b) in
   Bytes.hide v
 
 /// bytes wrapper for [EverCrypt.Hash.hash]
 val compute: a:alg -> text:hashable a -> Stack (tag a)
   (requires fun h0 -> True)
-  (ensures fun h0 t h1 -> 
-    let v = reveal text in 
+  (ensures fun h0 t h1 ->
+    let v = reveal text in
     B.modifies B.loc_none h0 h1 /\
-    Seq.length v <= maxLength a /\
+    Seq.length v <= max_input_length a /\
     t = h a text)
 
 #push-options "--max_fuel 0 --max_ifuel 0 --z3rlimit 40"
-let compute a text = 
-  let h00 = ST.get() in 
-  push_frame(); 
-  let tlen = EverCrypt.Hash.tagLen a in
+let compute a text =
+  let h00 = ST.get() in
+  push_frame();
+  let tlen = Hacl.Hash.Definitions.hash_len a in
   let output = LowStar.Buffer.alloca 0uy tlen in
-  let len = Bytes.len text in 
+  let len = Bytes.len text in
   if len = 0ul then (
-    let input = LowStar.Buffer.null in 
+    let input = LowStar.Buffer.null in
     //18-09-01 this could follow from LowStar.Buffer or Bytes properties
-    let h0 = ST.get() in 
+    let h0 = ST.get() in
     Seq.lemma_eq_intro (reveal text) (LowStar.Buffer.as_seq h0 input);
-    EverCrypt.Hash.hash a output input len 
+    EverCrypt.Hash.hash a output input len
     )
   else (
     let h0 = ST.get() in
     push_frame();
-    let input = LowStar.Buffer.alloca 0uy len in 
+    let input = LowStar.Buffer.alloca 0uy len in
     store_bytes text input;
     EverCrypt.Hash.hash a output input len;
     pop_frame()
@@ -60,7 +60,7 @@ let compute a text =
 #pop-options
 
 
-(* IMPLEMENTATION PLACEHOLDER, 
+(* IMPLEMENTATION PLACEHOLDER,
     simply buffering the bytes underneath *)
 
 // 18-08-29 TODO actually use EverCrypt's incremental API, but this
@@ -72,7 +72,7 @@ private type accv' (a:alg) =  | Inputs: b: hashable a -> accv' a
 abstract type accv (a:alg) = accv' a
 
 abstract val content: #a:alg -> accv a -> Tot (hashable a)
-let content #a v = 
+let content #a v =
   match v with Inputs b -> b
 
 abstract val start: a:alg -> Tot (v:accv a {content v == empty_bytes})
@@ -84,112 +84,112 @@ abstract val finalize: #a:alg -> v:accv a -> ST (t:tag a {t == h a (content v)})
 
 let start a = Inputs empty_bytes
 let extend #a (Inputs b0) b1 =
-  assume (FStar.UInt.fits (length b0 + length b1) 32); 
-  assume (length b0 + length b1 < Hashing.Spec.maxLength a); 
+  assume (FStar.UInt.fits (length b0 + length b1) 32);
+  assume (length b0 + length b1 < Hashing.Spec.max_input_length a);
   Inputs (b0 @| b1)
 let finalize #a (Inputs b) = compute a b
 
 (* older construction, still used in sig *)
-let compute_MD5SHA1 data = compute MD5 data @| compute SHA1 data 
+let compute_MD5SHA1 data = compute MD5 data @| compute SHA1 data
 
 (*
 // 18-08-29 was in Hashing.OpenSSL
-val hmac: 
-  a:alg -> 
-  k:tag a -> 
-  m:bytes {length m + blockLength a <= maxLength a } -> 
+val hmac:
+  a:alg ->
+  k:tag a ->
+  m:bytes {length m + block_length a <= max_input_length a } ->
   Stack (t:tag a {reveal t == Spec.HMAC.hmac a (reveal k) (reveal m)})
   (requires fun h0 -> True)
   (ensures fun h0 t h1 -> modifies Set.empty h0 h1)
 *)
 
-(* another PURE, VERIFIED, INCREMENTAL IMPLEMENTATION 
-    not usable yet, as we don't have a full F* specification 
+(* another PURE, VERIFIED, INCREMENTAL IMPLEMENTATION
+    not usable yet, as we don't have a full F* specification
     of the underlying core algorithms, or their OpenSSL code.
 
-// an "outer" state for specifying incremental evaluation 
+// an "outer" state for specifying incremental evaluation
 // (we may additionally record the input bytestring)
-noeq type accv (a:alg) = | Acc: 
+noeq type accv (a:alg) = | Acc:
     len:nat -> // total input length so far
-    v:acc a -> // current internal state 
-    b:lbytes (len % blockLen a) -> // pending bytes to be hashed  
-    accv a 
+    v:acc a -> // current internal state
+    b:lbytes (len % block_len a) -> // pending bytes to be hashed
+    accv a
 
 // the real state for our pure reference implementation
 // the ideal state may keep instead the whole input bytestring
 // or we could index this type with the whole input bytestring
 
-// incremental computation (specification) 
+// incremental computation (specification)
 val hashA: a:alg -> bytes -> Tot (accv a)
-let hashA a b = 
-  let pending = length b % blockLen a in 
+let hashA a b =
+  let pending = length b % block_len a in
   let hashed, rest = split b (length b - pending) in
   Acc (length b) (hash2 (acc0 a) hashed) rest
 
 let start a = hashA a empty_bytes // i.e. block0
 
 // this interface requires that the caller knows what he is hashing, to keep track of computed collisions
-val extend: 
+val extend:
   #a:alg ->
-  content:bytes (* TODO: ghost in real mode *) -> 
+  content:bytes (* TODO: ghost in real mode *) ->
   v:accv a {v == hashA a content } ->
   b:bytes ->
   Tot (v:accv a {v == hashA a (content @| b) })
 
-private assume val split_append: xs:bytes -> ys:bytes -> i:nat { i <= Seq.length xs } -> 
+private assume val split_append: xs:bytes -> ys:bytes -> i:nat { i <= Seq.length xs } ->
   Lemma(
     let c,b = split xs i in (split (xs@|ys) i == (c, (b@|ys))))
-  
+
 private val hash2_append:
   #a:alg ->
-  v:acc a  -> 
-  b0:bytes { length b0 % blockLen a = 0 } -> 
-  b1:bytes { length b1 % blockLen a = 0 } -> 
+  v:acc a  ->
+  b0:bytes { length b0 % block_len a = 0 } ->
+  b1:bytes { length b1 % block_len a = 0 } ->
   Lemma (ensures hash2 v (b0 @| b1) == hash2 (hash2 v b0) b1) (decreases (length b0))
-let rec hash2_append #a v b0 b1 = 
+let rec hash2_append #a v b0 b1 =
   if length b0 = 0 then (
     assert(Seq.equal b0 empty_bytes);
     assert(Seq.equal (b0 @| b1) b1);
     assert_norm(hash2 v empty_bytes == v))
-  else 
-    let c,b = split b0 (blockLen a) in
-    split_append b0 b1 (blockLen a); 
+  else
+    let c,b = split b0 (block_len a) in
+    split_append b0 b1 (block_len a);
     hash2_append (compress v c) b b1
-  
+
 #set-options "--z3rlimit 200"
-let extend #a content v b = 
-  let z = v.b @| b in 
-  let pending = length z % blockLen a in
+let extend #a content v b =
+  let z = v.b @| b in
+  let pending = length z % block_len a in
   let hashed, rest = split z (length z - pending) in
   // proof only: unfolding a == hashA content
-  assert(Seq.equal z (hashed @| rest)); 
-  let b0, c0 = split content (length content - (length content % blockLen a)) in 
+  assert(Seq.equal z (hashed @| rest));
+  let b0, c0 = split content (length content - (length content % block_len a)) in
   assert(Seq.equal content (b0 @| v.b));
   assert(v.len = length content);
   assert(v.v == hash2 (acc0 a) b0);
-  hash2_append (acc0 a) b0 hashed; 
-  let content' = content @| b in  // unfolding hashA (content @| b) 
-  let b0', c0' = split content' (length content' - (length content' % blockLen a)) in 
+  hash2_append (acc0 a) b0 hashed;
+  let content' = content @| b in  // unfolding hashA (content @| b)
+  let b0', c0' = split content' (length content' - (length content' % block_len a)) in
   assert(Seq.equal rest c0');
   assert(Seq.equal content' (b0' @| rest));
   assert(Seq.equal b0' (b0 @| hashed));
-  assert(pending = length content' % blockLen a);
+  assert(pending = length content' % block_len a);
   assert(v.len + length b = length (content @| b));
   assert(hash2 v.v hashed == hash2 (acc0 a) (b0 @| hashed));
   Acc (v.len + length b) (hash2 v.v hashed) rest
 
-val final: 
-  #a:alg -> 
+val final:
+  #a:alg ->
   content:bytes (* TODO: ghost in real mode *) ->
-  v:accv a { v == hashA a content } -> 
-  Tot (t:lbytes (tagLen a) {t = hash a content})
-  
-let final #a content v = 
-  let b0, rest = split content (length content - length content % blockLen a) in 
+  v:accv a { v == hashA a content } ->
+  Tot (t:lbytes (hash_len a) {t = hash a content})
+
+let final #a content v =
+  let b0, rest = split content (length content - length content % block_len a) in
   assert(Seq.equal content (b0 @| rest));
-  let b1 = v.b @| suffix a v.len in 
-  let b = content @| suffix a v.len in 
-  assert(Seq.equal b (b0 @| b1)); 
-  hash2_append (acc0 a) b0 b1; 
+  let b1 = v.b @| suffix a v.len in
+  let b = content @| suffix a v.len in
+  assert(Seq.equal b (b0 @| b1));
+  hash2_append (acc0 a) b0 b1;
   truncate (hash2 v.v b1)
 
