src/tls/CipherSuite.fsti
@@ -61,8 +61,8 @@ type hashAlg = Hashing.Spec.tls_alg
 type macAlg = Hashing.Spec.alg
 
 let hashSize = Hashing.Spec.tls_tagLen
-let macKeySize = Hashing.Spec.tagLen
-let macSize = Hashing.Spec.tagLen
+let macKeySize = Hacl.Hash.Definitions.hash_len
+let macSize = Hacl.Hash.Definitions.hash_len
 
 (** Authenticated Encryption modes *)
 type aeAlg =
