src/tls/KDF.fst
@@ -89,7 +89,7 @@ noeq private type table (#ideal:iflag) (u:usage ideal) (i:regid) (s:squash model
     table u i s
 
 inline_for_extraction
-let secret_len (a:info) : keylen = Hashing.Spec.tagLen a.ha
+let secret_len (a:info) : keylen = Hacl.Hash.Definitions.hash_len a.ha
 type real_secret (i:regid) = a:info0 i & lbytes32 (secret_len a)
 
 let safe (#ideal:iflag) (u:usage ideal) (i:regid) =
@@ -452,7 +452,7 @@ val derive:
   ST (_:squash (registered (derive i lbl ctx)) &
       (LocalPkg?.key child_pkg) (derive i lbl ctx))
   (requires fun h0 ->
-    (LocalPkg?.len child_pkg) a' == EverCrypt.Hash.tagLen (get_info k).ha /\
+    (LocalPkg?.len child_pkg) a' == Hacl.Hash.Definitions.hash_len (get_info k).ha /\
     ((u_of_t t) `has_lbl` lbl ==>
       compatible_packages child_pkg (child (u_of_t t) lbl)) /\
     mem_defined (kdf_dt t) i /\
